theories/HTactics.v
@@ -13,18 +13,21 @@ Require Import Relation_Operators.
 Require Import RelationPairs.
 From ExtLib Require Import
      Data.Map.FMapAList.
+From Ordinal Require Export Ordinal Arithmetic.
 
 Generalizable Variables E R A B C X Y Σ.
 
 Set Implicit Arguments.
 
-Hint Resolve sim_itree_mon: paco.
-Hint Resolve cpn6_wcompat: paco.
+#[export] Hint Resolve sim_itree_mon: paco.
+#[export] Hint Resolve cpn6_wcompat: paco.
+
+Create HintDb ord_step.
+#[export] Hint Resolve OrdArith.lt_from_nat OrdArith.lt_add_r Nat.lt_succ_diag_r: ord_step.
 
 Ltac anytac := (try rewrite ! Any.upcast_downcast in *); clarify; apply_all_once Any.upcast_inj; des; clarify; clear_tac.
 
 Ltac asimpl := try (unfold alist_add, alist_remove in *); ss.
-
 
 Section HOARE.
   Let Any_tgt := Any.t.
@@ -94,9 +97,9 @@ Section SIM.
   Variable wf: W -> Prop.
 
 
-  Variant _safe_sim_itree (sim_itree: forall (R_src R_tgt: Type) (RR: st_local -> st_local -> R_src -> R_tgt -> Prop), nat -> st_local * itree Es R_src -> st_local * itree Es R_tgt -> Prop)
+  Variant _safe_sim_itree (sim_itree: forall (R_src R_tgt: Type) (RR: st_local -> st_local -> R_src -> R_tgt -> Prop), Ord.t -> st_local * itree Es R_src -> st_local * itree Es R_tgt -> Prop)
           {R_src R_tgt} (RR: st_local -> st_local -> R_src -> R_tgt -> Prop)
-    : nat -> st_local * itree Es R_src -> st_local * itree Es R_tgt -> Prop :=
+    : Ord.t -> st_local * itree Es R_src -> st_local * itree Es R_tgt -> Prop :=
   | safe_sim_itree_ret
       i0 mrs_src0 mrs_tgt0 fr_src0 fr_tgt0
       (WF: wf (mrs_src0, mrs_tgt0))
@@ -133,14 +136,14 @@ Section SIM.
   | safe_sim_itree_tau_src
       i0 st_src0 st_tgt0
       i1 i_src i_tgt
-      (ORD: i1 < i0)
+      (ORD: (i1 < i0)%ord)
       (K: sim_itree _ _ RR i1 (st_src0, i_src) (st_tgt0, i_tgt))
     :
       _safe_sim_itree sim_itree RR i0 (st_src0, tau;; i_src) (st_tgt0, i_tgt)
   | safe_sim_itree_take_src
       i0 mrs_src0 mrs_tgt0 fr_src0 fr_tgt0
       i1 X k_src i_tgt
-      (ORD: i1 < i0)
+      (ORD: (i1 < i0)%ord)
       (K: forall (x: X), sim_itree _ _ RR i1 ((mrs_src0, fr_src0), k_src x) ((mrs_tgt0, fr_tgt0), i_tgt))
     :
       _safe_sim_itree sim_itree RR i0 ((mrs_src0, fr_src0), trigger (Take X) >>= k_src)
@@ -149,7 +152,7 @@ Section SIM.
   | safe_sim_itree_pput_src
       i0 mrs_src0 mrs_tgt0 fr_src0 fr_tgt0
       i1 k_src i_tgt
-      (ORD: i1 < i0)
+      (ORD: (i1 < i0)%ord)
       mn mr0 mp1 mrs_src1 mp0
       (MR0: Maps.lookup mn mrs_src0 = Some (mr0, mp0))
       (EQ: mrs_src1 = Maps.add mn (mr0, mp1) mrs_src0)
@@ -160,7 +163,7 @@ Section SIM.
   | safe_sim_itree_mput_src
       i0 mrs_src0 mrs_tgt0 fr_src0 fr_tgt0
       i1 k_src i_tgt
-      (ORD: i1 < i0)
+      (ORD: (i1 < i0)%ord)
       mn mr0 mr1 mrs_src1 mp0
       (MR0: Maps.lookup mn mrs_src0 = Some (mr0, mp0))
       (EQ: mrs_src1 = Maps.add mn (mr1, mp0) mrs_src0)
@@ -171,7 +174,7 @@ Section SIM.
   | safe_sim_itree_fput_src
       i0 mrs_src0 mrs_tgt0 fr_src0 fr_tgt0
       i1 k_src i_tgt
-      (ORD: i1 < i0)
+      (ORD: (i1 < i0)%ord)
       fr_src1
       (K: sim_itree _ _ RR i1 ((mrs_src0, fr_src1), k_src tt) ((mrs_tgt0, fr_tgt0), i_tgt))
     :
@@ -181,7 +184,7 @@ Section SIM.
   | safe_sim_itree_pget_src
       i0 mrs_src0 mrs_tgt0 fr_src0 fr_tgt0
       i1 k_src i_tgt
-      (ORD: i1 < i0)
+      (ORD: (i1 < i0)%ord)
       mn mr0 mp0
       (MR0: Maps.lookup mn mrs_src0 = Some (mr0, mp0))
       (K: sim_itree _ _ RR i1 ((mrs_src0, fr_src0), k_src mp0) ((mrs_tgt0, fr_tgt0), i_tgt))
@@ -191,7 +194,7 @@ Section SIM.
   | safe_sim_itree_mget_src
       i0 mrs_src0 mrs_tgt0 fr_src0 fr_tgt0
       i1 k_src i_tgt
-      (ORD: i1 < i0)
+      (ORD: (i1 < i0)%ord)
       mn mr0 mp0
       (MR0: Maps.lookup mn mrs_src0 = Some (mr0, mp0))
       (K: sim_itree _ _ RR i1 ((mrs_src0, fr_src0), k_src mr0) ((mrs_tgt0, fr_tgt0), i_tgt))
@@ -201,7 +204,7 @@ Section SIM.
   | safe_sim_itree_fget_src
       i0 mrs_src0 mrs_tgt0 fr_src0 fr_tgt0
       i1 k_src i_tgt
-      (ORD: i1 < i0)
+      (ORD: (i1 < i0)%ord)
       (K: sim_itree _ _ RR i1 ((mrs_src0, fr_src0), k_src fr_src0) ((mrs_tgt0, fr_tgt0), i_tgt))
     :
       _safe_sim_itree sim_itree RR i0 ((mrs_src0, fr_src0), trigger (FGet) >>= k_src)
@@ -210,14 +213,14 @@ Section SIM.
   | safe_sim_itree_tau_tgt
       i0 st_src0 st_tgt0
       i1 i_src i_tgt
-      (ORD: i1 < i0)
+      (ORD: (i1 < i0)%ord)
       (K: sim_itree _ _ RR i1 (st_src0, i_src) (st_tgt0, i_tgt))
     :
       _safe_sim_itree sim_itree RR i0 (st_src0, i_src) (st_tgt0, tau;; i_tgt)
   | safe_sim_itree_choose_tgt
       i0 mrs_src0 mrs_tgt0 fr_src0 fr_tgt0
       i1 X i_src k_tgt
-      (ORD: i1 < i0)
+      (ORD: (i1 < i0)%ord)
       (K: forall (x: X), sim_itree _ _ RR i1 ((mrs_src0, fr_src0), i_src) ((mrs_tgt0, fr_tgt0), k_tgt x))
     :
       _safe_sim_itree sim_itree RR i0 ((mrs_src0, fr_src0), i_src)
@@ -226,7 +229,7 @@ Section SIM.
   | safe_sim_itree_pput_tgt
       i0 mrs_src0 mrs_tgt0 fr_src0 fr_tgt0
       i1 i_src k_tgt
-      (ORD: i1 < i0)
+      (ORD: (i1 < i0)%ord)
       mn mr0 mp1 mrs_tgt1 mp0
       (MR0: Maps.lookup mn mrs_tgt0 = Some (mr0, mp0))
       (EQ: mrs_tgt1 = Maps.add mn (mr0, mp1) mrs_tgt0)
@@ -237,7 +240,7 @@ Section SIM.
   | safe_sim_itree_mput_tgt
       i0 mrs_src0 mrs_tgt0 fr_src0 fr_tgt0
       i1 i_src k_tgt
-      (ORD: i1 < i0)
+      (ORD: (i1 < i0)%ord)
       mn mr0 mr1 mrs_tgt1 mp0
       (MR0: Maps.lookup mn mrs_tgt0 = Some (mr0, mp0))
       (EQ: mrs_tgt1 = Maps.add mn (mr1, mp0) mrs_tgt0)
@@ -248,7 +251,7 @@ Section SIM.
   | safe_sim_itree_fput_tgt
       i0 mrs_src0 mrs_tgt0 fr_src0 fr_tgt0
       i1 i_src k_tgt
-      (ORD: i1 < i0)
+      (ORD: (i1 < i0)%ord)
       fr_tgt1
       (K: sim_itree _ _ RR i1 ((mrs_src0, fr_src0), i_src) ((mrs_tgt0, fr_tgt1), k_tgt tt))
     :
@@ -258,7 +261,7 @@ Section SIM.
   | safe_sim_itree_pget_tgt
       i0 mrs_src0 mrs_tgt0 fr_src0 fr_tgt0
       i1 i_src k_tgt
-      (ORD: i1 < i0)
+      (ORD: (i1 < i0)%ord)
       mn mr0 mp0
       (MR0: Maps.lookup mn mrs_tgt0 = Some (mr0, mp0))
       (K: sim_itree _ _ RR i1 ((mrs_src0, fr_src0), i_src) ((mrs_tgt0, fr_tgt0), k_tgt mp0))
@@ -268,7 +271,7 @@ Section SIM.
   | safe_sim_itree_mget_tgt
       i0 mrs_src0 mrs_tgt0 fr_src0 fr_tgt0
       i1 i_src k_tgt
-      (ORD: i1 < i0)
+      (ORD: (i1 < i0)%ord)
       mn mr0 mp0
       (MR0: Maps.lookup mn mrs_tgt0 = Some (mr0, mp0))
       (K: sim_itree _ _ RR i1 ((mrs_src0, fr_src0), i_src) ((mrs_tgt0, fr_tgt0), k_tgt mr0))
@@ -278,7 +281,7 @@ Section SIM.
   | safe_sim_itree_fget_tgt
       i0 mrs_src0 mrs_tgt0 fr_src0 fr_tgt0
       i1 i_src k_tgt
-      (ORD: i1 < i0)
+      (ORD: (i1 < i0)%ord)
       (K: sim_itree _ _ RR i1 ((mrs_src0, fr_src0), i_src) ((mrs_tgt0, fr_tgt0), k_tgt  fr_tgt0))
     :
       _safe_sim_itree sim_itree RR i0 ((mrs_src0, fr_src0), i_src)
@@ -299,6 +302,8 @@ Ltac init :=
   split; ss; ii; clarify; rename y into varg; eexists 100%nat; ss; des; clarify;
   ginit; asimpl;
   try (unfold fun_to_tgt, cfun; rewrite HoareFun_parse); ss.
+
+(* TODO: init with user given ordinal *)
 
 Lemma sim_l_bind_bind `{Σ: GRA.t}
       (R S R_src R_tgt: Type) (RR: _ -> _ -> R_src -> R_tgt -> Prop)
@@ -458,10 +463,10 @@ Ltac force_l :=
     let thyp := fresh "TMP" in
     remember (guarantee P) as tvar eqn:thyp; unfold guarantee in thyp; subst tvar;
     let name := fresh "_GUARANTEE" in
-    destruct (classic P) as [name|name]; [ired_all; gstep; eapply sim_itree_choose_src; [eauto|exists name]|contradict name]; cycle 1
+    destruct (classic P) as [name|name]; [ired_all; gstep; eapply sim_itree_choose_src; [eauto with ord_step|exists name]|contradict name]; cycle 1
 
   | [ |- (gpaco6 (_sim_itree _) _ _ _ _ _ _ _ (_, ?i_src) (_, ?i_tgt)) ] =>
-    seal i_tgt; gstep; econs; eauto; unseal i_tgt
+    seal i_tgt; gstep; econs; eauto with ord_step; unseal i_tgt
   end
 .
 
@@ -479,10 +484,10 @@ Ltac force_r :=
     let thyp := fresh "TMP" in
     remember (assume P) as tvar eqn:thyp; unfold assume in thyp; subst tvar;
     let name := fresh "_ASSUME" in
-    destruct (classic P) as [name|name]; [ired_all; gstep; eapply sim_itree_take_tgt; [eauto|exists name]|contradict name]; cycle 1
+    destruct (classic P) as [name|name]; [ired_all; gstep; eapply sim_itree_take_tgt; [eauto with ord_step|exists name]|contradict name]; cycle 1
 
   | [ |- (gpaco6 (_sim_itree _) _ _ _ _ _ _ _ (_, ?i_src) (_, ?i_tgt)) ] =>
-    seal i_src; gstep; econs; eauto; unseal i_src
+    seal i_src; gstep; econs; eauto with ord_step; unseal i_src
   end
 .
 
@@ -501,7 +506,7 @@ Ltac _step :=
     let thyp := fresh "TMP" in
     remember (assume P) as tvar eqn:thyp; unfold assume in thyp; subst tvar;
     let name := fresh "_ASSUME" in
-    ired_all; gstep; eapply sim_itree_take_src; [apply Nat.lt_succ_diag_r|]; intro name
+    ired_all; gstep; eapply sim_itree_take_src; [eapply OrdArith.lt_from_nat; apply Nat.lt_succ_diag_r|]; intro name
 
   (*** blacklisting ***)
   (* | [ |- (gpaco5 (_sim_itree wf) _ _ _ _ (_, _) (_, trigger (Take _) >>= _)) ] => idtac *)
@@ -516,12 +521,12 @@ Ltac _step :=
     let thyp := fresh "TMP" in
     remember (guarantee P) as tvar eqn:thyp; unfold guarantee in thyp; subst tvar;
     let name := fresh "_GUARANTEE" in
-    ired_all; gstep; eapply sim_itree_choose_tgt; [apply Nat.lt_succ_diag_r|]; intro name
+    ired_all; gstep; eapply sim_itree_choose_tgt; [eapply OrdArith.lt_from_nat; apply Nat.lt_succ_diag_r|]; intro name
 
 
 
   | _ => (*** default ***)
-    gstep; eapply safe_sim_sim; econs; try apply Nat.lt_succ_diag_r; i
+    gstep; eapply safe_sim_sim; econs; try (eapply OrdArith.lt_from_nat; apply Nat.lt_succ_diag_r); i
   end;
   (* idtac *)
   match goal with
@@ -541,6 +546,76 @@ Section HLEMMAS.
   Context `{Σ: GRA.t}.
   Local Opaque GRA.to_URA.
 
+  Lemma hcall_clo_ord (o_new: Ord.t)
+        X (x: X) (o: ord)
+        (mr_src1 fr_src1 rarg_src: Σ)
+        r rg (n: nat) mr_src0 mp_src0 fr_src0 Y Z
+        (P: X -> Y -> Any.t -> ord -> Σ -> Prop)
+        (Q: X -> Z -> Any.t -> Σ -> Prop)
+        mrs_tgt frs_tgt k_tgt k_src
+        mn fn tbr ord_cur varg_src varg_tgt
+        (wf: (alist mname (Σ * Any.t)) * (alist mname (Σ * Any.t)) -> Prop)
+
+        (UPDATABLE: URA.updatable (URA.add mr_src0 fr_src0) (URA.add mr_src1 (URA.add rarg_src fr_src1)))
+        (FUEL: (15 < n)%ord)
+        (PRE: P x varg_src varg_tgt o rarg_src)
+        (PURE: ord_lt o ord_cur /\
+               (tbr = true -> is_pure o) /\ (tbr = false -> o = ord_top))
+        (WF: wf ([(mn, (mr_src1, mp_src0))], mrs_tgt))
+        (POST: forall (vret_tgt : Any.t) (mrs_src1 mrs_tgt1 : alist string (Σ * Any.t))
+                      (rret: Σ) (vret_src: Z)
+                      (WF: wf (mrs_src1, mrs_tgt1)),
+            exists (mr_src2: Σ) (mp_src2: Any.t),
+              (<<LOOKUP: lookup mn mrs_src1 = Some (mr_src2, mp_src2)>>) /\
+              forall (VALID: URA.wf (URA.add mr_src2 (URA.add fr_src1 rret)))
+                     (POST: Q x vret_src vret_tgt rret),
+                gpaco6 (_sim_itree wf) (cpn6 (_sim_itree wf)) rg rg _ _ (fun _ _ => @eq Any.t) o_new
+                       (mrs_src1, URA.add fr_src1 rret, k_src vret_src) (mrs_tgt1, frs_tgt, k_tgt vret_tgt))
+    :
+      gpaco6 (_sim_itree wf) (cpn6 (_sim_itree wf)) r rg _ _ (fun _ _ => @eq Any.t) n
+             (([(mn, (mr_src0, mp_src0))], fr_src0),
+              (HoareCall mn tbr ord_cur P Q fn varg_src) >>= k_src)
+             ((mrs_tgt, frs_tgt),
+              trigger (Call fn varg_tgt) >>= k_tgt).
+  Proof.
+    unfold HoareCall, put, discard, forge, checkWf, assume, guarantee.
+    ired. gstep. econs; eauto with ord_step. exists (mr_src1, URA.add rarg_src fr_src1).
+    ired. gstep. econs; eauto with ord_step.
+    { instantiate (1:=mp_src0). instantiate (1:=mr_src0). admit "ez". }
+    ired. gstep. econs; eauto with ord_step.
+    ired. gstep. econs; eauto with ord_step. split; auto.
+    ired. gstep. econs; eauto with ord_step.
+    ired. gstep. econs; eauto with ord_step.
+    { instantiate (1:=mp_src0). instantiate (1:=mr_src0). admit "ez". }
+    ired. gstep. econs; eauto with ord_step. exists rarg_src.
+    ired. gstep. econs; eauto with ord_step.
+    replace (alist_add Dec_RelDec mn (mr_src1, mp_src0) [(mn, (mr_src0, mp_src0))]) with [(mn, (mr_src1, mp_src0))].
+    2: { admit "ez". }
+    ired. gstep. econs; eauto with ord_step. exists fr_src1.
+    ired. gstep. econs; eauto with ord_step. split; auto.
+    ired. gstep. econs; eauto with ord_step.
+    ired. gstep. econs; eauto with ord_step. exists x.
+    ired. gstep. econs; eauto with ord_step. exists varg_tgt.
+    ired. gstep. econs; eauto with ord_step. exists o.
+    ired. gstep. econs; eauto with ord_step. split; auto.
+    ired. gstep. econs; eauto with ord_step. split; auto.
+    ired. gstep. econs; eauto with ord_step. i. exists (o_new + 8)%ord.
+    ired. gstep. econs; eauto with ord_step. i.
+    ired. gstep. econs; eauto with ord_step.
+    ired. gstep. econs; eauto with ord_step.
+    ired. gstep. econs; eauto with ord_step. i.
+    hexploit (POST vret mrs_src1 mrs_tgt1 x0 x1 WF0). i. des.
+    ired. gstep. econs; eauto with ord_step.
+    ired. gstep. econs; eauto with ord_step.
+    ired. gstep. econs; eauto with ord_step. i.
+    ired. gstep. econs.
+    { instantiate (1:=o_new). eapply Ord.eq_lt_lt.
+      { symmetry. eapply OrdArith.add_O_r. }
+      { eapply OrdArith.lt_add_r. rewrite Ord.from_nat_S. eapply Ord.S_pos. }
+    }
+    { eauto. }
+  Qed.
+
   Lemma hcall_clo
         X (x: X) (o: ord)
         (mr_src1 fr_src1 rarg_src: Σ)
@@ -552,7 +627,7 @@ Section HLEMMAS.
         (wf: (alist mname (Σ * Any.t)) * (alist mname (Σ * Any.t)) -> Prop)
 
         (UPDATABLE: URA.updatable (URA.add mr_src0 fr_src0) (URA.add mr_src1 (URA.add rarg_src fr_src1)))
-        (FUEL: n > 15)
+        (FUEL: (15 < n)%ord)
         (PRE: P x varg_src varg_tgt o rarg_src)
         (PURE: ord_lt o ord_cur /\
                (tbr = true -> is_pure o) /\ (tbr = false -> o = ord_top))
@@ -573,37 +648,7 @@ Section HLEMMAS.
              ((mrs_tgt, frs_tgt),
               trigger (Call fn varg_tgt) >>= k_tgt).
   Proof.
-    unfold HoareCall, put, discard, forge, checkWf, assume, guarantee.
-    ired. gstep. econs; eauto. exists (mr_src1, URA.add rarg_src fr_src1).
-    ired. gstep. econs; eauto.
-    { instantiate (1:=mp_src0). instantiate (1:=mr_src0). admit "ez". }
-    ired. gstep. econs; eauto.
-    ired. gstep. econs; eauto. split; auto.
-    ired. gstep. econs; eauto.
-    ired. gstep. econs; eauto.
-    { instantiate (1:=mp_src0). instantiate (1:=mr_src0). admit "ez". }
-    ired. gstep. econs; eauto. exists rarg_src.
-    ired. gstep. econs; eauto.
-    replace (alist_add Dec_RelDec mn (mr_src1, mp_src0) [(mn, (mr_src0, mp_src0))]) with [(mn, (mr_src1, mp_src0))].
-    2: { admit "ez". }
-    ired. gstep. econs; eauto. exists fr_src1.
-    ired. gstep. econs; eauto. split; auto.
-    ired. gstep. econs; eauto.
-    ired. gstep. econs; eauto. exists x.
-    ired. gstep. econs; eauto. exists varg_tgt.
-    ired. gstep. econs; eauto. exists o.
-    ired. gstep. econs; eauto. split; auto.
-    ired. gstep. econs; eauto. split; auto.
-    ired. gstep. econs; eauto. i. exists 108.
-    ired. gstep. econs; eauto. i.
-    ired. gstep. econs; eauto.
-    ired. gstep. econs; eauto.
-    ired. gstep. econs; eauto. i.
-    hexploit (POST vret mrs_src1 mrs_tgt1 x0 x1 WF0). i. des.
-    ired. gstep. econs; eauto.
-    ired. gstep. econs; eauto.
-    ired. gstep. econs; eauto. i.
-    ired. gstep. econs; eauto.
+    eapply (@hcall_clo_ord 100); eauto.
   Qed.
 
   Lemma harg_clo
@@ -626,17 +671,17 @@ Section HLEMMAS.
               f_tgt).
   Proof.
     unfold HoareFunArg, put, discard, forge, checkWf, assume, guarantee.
-    ired. gstep. econs; eauto. intros varg_src.
-    ired. gstep. econs; eauto. intros x.
-    ired. gstep. econs; eauto. intros rarg_src.
-    ired. gstep. econs; eauto.
-    ired. gstep. econs; eauto.
-    ired. gstep. econs; eauto.
+    ired. gstep. econs; eauto with ord_step. intros varg_src.
+    ired. gstep. econs; eauto with ord_step. intros x.
+    ired. gstep. econs; eauto with ord_step. intros rarg_src.
+    ired. gstep. econs; eauto with ord_step.
+    ired. gstep. econs; eauto with ord_step.
+    ired. gstep. econs; eauto with ord_step.
     { instantiate (1:=mp_src0). instantiate (1:=mr_src0). admit "ez". }
-    ired. gstep. econs; eauto.
-    ired. gstep. econs; eauto. intros VALID.
-    ired. gstep. econs; eauto. intros ord_cur.
-    ired. gstep. econs; eauto.
+    ired. gstep. econs; eauto with ord_step.
+    ired. gstep. econs; eauto with ord_step. intros VALID.
+    ired. gstep. econs; eauto with ord_step. intros ord_cur.
+    ired. gstep. econs; eauto with ord_step.
   Qed.
 
   Lemma hret_clo (mr_src1 rret_src: Σ)
@@ -645,7 +690,7 @@ Section HLEMMAS.
         x vret_src vret_tgt
         mrs_tgt frs_tgt
         (wf: (alist mname (Σ * Any.t)) * (alist mname (Σ * Any.t)) -> Prop)
-        (FUEL: n > 14)
+        (FUEL: (14 < n)%ord)
         (UPDATABLE: URA.updatable (URA.add mr_src0 fr_src0) (URA.add mr_src1 rret_src))
         (POST: Q x vret_src vret_tgt rret_src)
         (WF: wf ([(mn, (mr_src1, mp_src0))], mrs_tgt))
@@ -657,23 +702,23 @@ Section HLEMMAS.
               (Ret vret_tgt)).
   Proof.
     unfold HoareFunRet, put, discard, forge, checkWf, assume, guarantee.
-    ired. gstep. econs; eauto. exists vret_tgt.
-    ired. gstep. econs; eauto. exists (mr_src1, rret_src).
-    ired. gstep. econs; eauto.
+    ired. gstep. econs; eauto with ord_step. exists vret_tgt.
+    ired. gstep. econs; eauto with ord_step. exists (mr_src1, rret_src).
+    ired. gstep. econs; eauto with ord_step.
     { instantiate (1:=mp_src0). instantiate (1:=mr_src0). admit "ez". }
-    ired. gstep. econs; eauto.
-    ired. gstep. econs; eauto. split; auto.
-    ired. gstep. econs; eauto.
-    ired. gstep. econs; eauto.
+    ired. gstep. econs; eauto with ord_step.
+    ired. gstep. econs; eauto with ord_step. split; auto.
+    ired. gstep. econs; eauto with ord_step.
+    ired. gstep. econs; eauto with ord_step.
     { instantiate (1:=mp_src0). instantiate (1:=mr_src0). admit "ez". }
-    ired. gstep. econs; eauto. exists rret_src.
-    ired. gstep. econs; eauto. split; auto.
-    ired. gstep. econs; eauto.
-    ired. gstep. econs; eauto. exists ε.
-    ired. gstep. econs; eauto. split.
+    ired. gstep. econs; eauto with ord_step. exists rret_src.
+    ired. gstep. econs; eauto with ord_step. split; auto.
+    ired. gstep. econs; eauto with ord_step.
+    ired. gstep. econs; eauto with ord_step. exists ε.
+    ired. gstep. econs; eauto with ord_step. split.
     { rewrite URA.unit_id. auto. }
-    ired. gstep. econs; eauto.
-    ired. gstep. econs; eauto.
+    ired. gstep. econs; eauto with ord_step.
+    ired. gstep. econs; eauto with ord_step.
     replace (alist_add Dec_RelDec mn (mr_src1, mp_src0) [(mn, (mr_src0, mp_src0))]) with [(mn, (mr_src1, mp_src0))].
     2: { admit "ez". }
     auto.
@@ -682,9 +727,9 @@ End HLEMMAS.
 
 Ltac _harg_tac := prep; eapply harg_clo; i.
 
-Ltac _hcall_tac x o mr_src1 fr_src1 rarg_src := prep; eapply (@hcall_clo _ _ x o mr_src1 fr_src1 rarg_src); [|lia|..].
+Ltac _hcall_tac x o mr_src1 fr_src1 rarg_src := prep; eapply (@hcall_clo _ _ x o mr_src1 fr_src1 rarg_src); [|eapply OrdArith.lt_from_nat; lia|..].
 
-Ltac _hret_tac mr_src1 rret_src := prep; eapply (@hret_clo _ mr_src1 rret_src); [lia|..].
+Ltac _hret_tac mr_src1 rret_src := prep; eapply (@hret_clo _ mr_src1 rret_src); [eapply OrdArith.lt_from_nat; lia|..].
 
 Require Import TODOYJ Logic YPM.
 
@@ -713,10 +758,10 @@ Ltac hcall_tac x o MR_SRC1 FR_SRC1 RARG_SRC :=
   match x with
   | ltac_wild =>
     match o with
-    | ltac_wild => eapply (hcall_clo _ (mr_src1:=mr_src1) (fr_src1:=fr_src1) (rarg_src:=rarg_src)); [tac0|lia|..|tac1]
-    | _ => eapply (hcall_clo _ (o:=o) (mr_src1:=mr_src1) (fr_src1:=fr_src1) (rarg_src:=rarg_src)); [tac0|lia|..|tac1]
+    | ltac_wild => eapply (hcall_clo _ (mr_src1:=mr_src1) (fr_src1:=fr_src1) (rarg_src:=rarg_src)); [tac0|eapply OrdArith.lt_from_nat; lia|..|tac1]
+    | _ => eapply (hcall_clo _ (o:=o) (mr_src1:=mr_src1) (fr_src1:=fr_src1) (rarg_src:=rarg_src)); [tac0|eapply OrdArith.lt_from_nat; lia|..|tac1]
     end
-  | _ => eapply (hcall_clo x (o:=o) (mr_src1:=mr_src1) (fr_src1:=fr_src1) (rarg_src:=rarg_src)); [tac0|lia|..|tac1]
+  | _ => eapply (hcall_clo x (o:=o) (mr_src1:=mr_src1) (fr_src1:=fr_src1) (rarg_src:=rarg_src)); [tac0|eapply OrdArith.lt_from_nat; lia|..|tac1]
   end
 .
 
